IMP--_To_SAS+/Correctness.thy
@@ -1,0 +1,112 @@
+\<^marker>\<open>creator Florian Keßler\<close>
+
+section "Correctness"
+
+theory Correctness imports Reduction
+begin
+
+definition imp_minus_sas_plus_equivalent_states :: "com \<Rightarrow> com \<Rightarrow> nat \<Rightarrow> imp_state \<Rightarrow> sas_state \<Rightarrow> bool" where
+"imp_minus_sas_plus_equivalent_states c c1 r is ss = (ss PC = Some (Num (index_of (all_subprograms c) c1)) 
+  \<and> list_all (\<lambda>v. ss (VN v) = Some (Num (is v)) \<or> (is v > r \<and> ss (VN v) = Some \<omega>)) (enumerate_variables c))"  
+
+lemma imp_minus_sas_plus_equivalent_states_assign:
+  assumes "t' \<le> t"
+    "imp_minus_sas_plus_equivalent_states c (x ::= a) (t' * max_constant c) s ss1"
+  shows "imp_minus_sas_plus_equivalent_states c SKIP ((t' - Suc 0) * max_constant c)
+     (\<lambda>y. if y = x then aval a s else s y)
+     (ss1(VN x \<mapsto> Num (aval a s), PC \<mapsto> Num (index_of (all_subprograms c) SKIP)))"
+proof -
+  let ?ss2 = "ss1(VN x \<mapsto> Num (t * max_constant c), PC \<mapsto> Num (index_of (all_subprograms c) SKIP))"
+  let ?is2 = "\<lambda>a. if a = x then aval (A (N (t * max_constant c))) s else s a"
+  let ?r1 = "t' * max_constant c"
+  let ?r2 = "(t' - Suc 0) * max_constant c"
+  have "v \<in> set (enumerate_variables c)
+     \<Longrightarrow> ?ss2 (VN v) = Some (Num (?is2 v)) \<or> (?is2 v > ?r2 \<and> ?ss2 (VN v) = Some \<omega>)" for v 
+  proof -
+    assume "v \<in> set (enumerate_variables c)"
+    moreover have "list_all (\<lambda>v. ss1 (VN v) 
+      = Some (Num (s v)) \<or> (s v > ?r1 \<and> ss1 (VN v) = Some \<omega>)) (enumerate_variables c)"
+      using assms by(auto simp: imp_minus_sas_plus_equivalent_states_def)
+    ultimately have "ss1 (VN v) = Some (Num (s v)) \<or> (s v > ?r1 \<and> ss1 (VN v) = Some \<omega>)" 
+      by (simp add: list_all_iff)
+    then show ?thesis using diff_mult_distrib by auto
+  qed
+  then show ?thesis using assms 
+    by (fastforce simp: imp_minus_sas_plus_equivalent_states_def list_all_iff)
+qed
+
+lemma "a \<noteq> c \<Longrightarrow> f(a \<mapsto> b, c \<mapsto> d) = (\<lambda>x. if x = a then Some b else (f(c \<mapsto> d)) x)" 
+  by auto
+
+
+lemma imp_minus_minus_to_sas_plus_single_step:
+   "(c1, is1) \<rightarrow> (c2, is2) \<Longrightarrow> cs = all_subprograms c \<Longrightarrow> c1 \<in> set cs \<Longrightarrow> t' \<le> t \<Longrightarrow> t > 0
+  \<Longrightarrow> imp_minus_sas_plus_equivalent_states c c1 (t' *  (max_constant c)) is1 ss1 
+  \<Longrightarrow> (\<exists>op \<in> set (com_to_operators cs c1 (domain c t)). \<exists>ss2.
+     imp_minus_sas_plus_equivalent_states c c2 ((t' - 1) *  (max_constant c)) is2 ss2
+    \<and> is_operator_applicable_in ss1 op
+    \<and> execute_operator_sas_plus ss1 op = ss2)"
+proof (induction c1 is1 c2 is2 rule: small_step_induct)
+  case (Assign x a s)
+  let ?i = "index_of cs (x ::= a)"
+  let ?j = "index_of cs SKIP"
+  have "SKIP \<in> set (all_subprograms c)" using SKIP_in_enumerate_subprograms by simp
+  moreover then have "SKIP \<in> set cs" using Assign by blast
+  have "aval a s \<le> t * (max_constant c) \<or> aval a s > t * (max_constant c)" by auto
+  show ?case
+  proof (cases a)
+    case (A atom)
+    then show ?thesis
+    proof (cases atom)
+      case (N val)
+      let ?op = "\<lparr> precondition_of = [(PC, Num ?i)], 
+                  effect_of = [(PC, Num ?j), (VN x, (if val \<le> t * (max_constant c) then Num val else \<omega>))]\<rparr>"
+      let ?ss2 = "ss1(VN x \<mapsto> Num val, PC \<mapsto> Num ?j)"
+      have "val \<le> max_constant c" using enumerate_subprograms_max_constant Assign A N by fastforce
+      then have "Num val \<in> set (domain c t)" using Assign by (auto simp: domain_def Let_def) 
+          (metis Suc_lessI add.right_neutral atLeastLessThan_iff image_eqI lambda_zero le_0_eq le_less_trans le_neq_implies_less n_less_m_mult_n nat_le_linear times_nat.simps(2))
+      moreover have "?op \<in> set (com_to_operators cs (x ::= a) (domain c t))" 
+        using A N by (auto simp: domain_def Let_def)
+      moreover have "is_operator_applicable_in ss1 ?op" using Assign 
+        by (auto simp: imp_minus_sas_plus_equivalent_states_def)
+           (metis (no_types) fun_upd_triv map_le_empty map_le_upd)
+      moreover have "imp_minus_sas_plus_equivalent_states c SKIP ((t' - Suc 0) * max_constant c) 
+        (\<lambda>y. if y = x then val else s y)
+        ?ss2" using Assign A N 
+        by (smt atomVal.simps aval.simps imp_minus_sas_plus_equivalent_states_def list_all_iff imp_minus_sas_plus_equivalent_states_assign[OF Assign(3) Assign(5)])
+      moreover have "ss1(VN x \<mapsto> Num val, PC \<mapsto> Num (index_of (all_subprograms c) SKIP)) 
+        = (\<lambda>a. if a = PC then Some (Num (index_of (all_subprograms c) SKIP)) else (ss1(VN x \<mapsto> Num val)) a)" by auto
+      ultimately show ?thesis using Assign A N by (simp add: domain_def Let_def)
+    next
+      case (V var)
+      then show ?thesis sorry
+    qed
+  next
+    case (Plus x21 x22)
+    then show ?thesis sorry
+  next
+    case (Sub x31 x32)
+    then show ?thesis sorry
+  qed
+next
+  case (Seq1 c\<^sub>2 s)
+  then show ?case sorry
+next
+  case (Seq2 c\<^sub>1 s c\<^sub>1' s' c\<^sub>2)
+  then show ?case sorry
+next
+  case (IfTrue s b c\<^sub>1 c\<^sub>2)
+  then show ?case sorry
+next
+  case (IfFalse s b c\<^sub>1 c\<^sub>2)
+  then show ?case sorry
+next
+  case (WhileTrue s b c)
+  then show ?case sorry
+next
+  case (WhileFalse s b c)
+  then show ?case sorry
+qed
+      
+
+end
